more examples

Examples/runtimes/net/src/Examples.cs
@@ -1,26 +1,33 @@
-﻿
-using Amazon.DynamoDBv2;
-using Amazon.DynamoDBv2.Model;
-using System.Threading.Tasks;
-using System;
+﻿using System;
 using System.Threading;
-using AWS.Cryptography.DbEncryptionSDK;
+using System.Threading.Tasks;
 
 namespace Examples
 {
-  class Program
-  {
-    // Main method
-    static async Task Main(string[] args)
+    class Program
     {
-      await BasicPutGetExample.PutItemGetItem();
-      var keyId = CreateKeyStoreKeyExample.KeyStoreCreateKey();
-      Thread.Sleep(5000);
-      await BasicSearchableEncryptionExample.PutItemQueryItemWithBeacon(keyId);
-      await CompoundBeaconSearchableEncryptionExample.PutItemQueryItemWithCompoundBeacon(keyId);
-      await VirtualBeaconSearchableEncryptionExample.PutItemQueryItemWithVirtualBeacon(keyId);
-      await BeaconStylesSearchableEncryptionExample.PutItemQueryItemWithBeaconStyles(keyId);
-      Console.Write("All examples completed successfully.\n");
+        // Main method
+        static async Task Main(string[] args)
+        {
+            ItemEncryptDecryptExample.PutItemGetItem();
+
+            await BasicPutGetExample.PutItemGetItem();
+           // await ClientSupplierExample.ClientSupplierPutItemGetItem();
+
+            var keyId = CreateKeyStoreKeyExample.KeyStoreCreateKey();
+            var keyId2 = CreateKeyStoreKeyExample.KeyStoreCreateKey();
+            // Key creation is eventually consistent, so wait 5 seconds to decrease the likelihood
+            // our test fails due to eventual consistency issues.
+            Thread.Sleep(5000);
+
+            await HierarchicalKeyringExample.HierarchicalKeyringGetItemPutItem(keyId, keyId2);
+            await MultiMrkKeyringExample.MultiMrkKeyringGetItemPutItem();
+            
+            await BasicSearchableEncryptionExample.PutItemQueryItemWithBeacon(keyId);
+            await CompoundBeaconSearchableEncryptionExample.PutItemQueryItemWithCompoundBeacon(keyId);
+            await VirtualBeaconSearchableEncryptionExample.PutItemQueryItemWithVirtualBeacon(keyId);
+            await BeaconStylesSearchableEncryptionExample.PutItemQueryItemWithBeaconStyles(keyId);
+            Console.Write("All examples completed successfully.\n");
+        }
     }
-  }
 }
