Examples/runtimes/net/src/itemencryptor/ItemEncryptDecryptExample.cs
@@ -1,32 +1,36 @@
 using System;
 using System.Collections.Generic;
 using System.Diagnostics;
-using System.Net;
-using System.Threading.Tasks;
 using Amazon.DynamoDBv2.Model;
-using AWS.Cryptography.DbEncryptionSDK.DynamoDb;
+using AWS.Cryptography.DbEncryptionSDK.DynamoDb.ItemEncryptor;
 using AWS.Cryptography.DbEncryptionSDK.StructuredEncryption;
 using AWS.Cryptography.MaterialProviders;
 
 /*
-  This example sets up DynamoDb Encryption for the AWS SDK client
-  and uses the low level PutItem and GetItem DDB APIs to demonstrate
-  putting a client-side encrypted item into DynamoDb
-  and then retrieving and decrypting that item from DynamoDb. 
+  This example sets up a DynamoDb Item Encryptor and uses
+  the EncryptItem and DecryptItem APIs to directly encrypt and
+  decrypt an existing DynamoDb item.
+  You should use the DynamoDb Item Encryptor
+  if you already have a DynamoDb Item to encrypt or decrypt,
+  and do not need to make a Put or Get call to DynamoDb.
+  For example, if you are using DynamoDb Streams,
+  you may already be working with an encrypted item obtained from
+  DynamoDb, and want to directly decrypt the item.
 
   Running this example requires access to the DDB Table whose name
   is provided in CLI arguments.
   This table must be configured with the following
   primary key configuration:
     - Partition key is named "partition_key" with type (S)
-    - Sort key is named "sort_key" with type (N)
+    - Sort key is named "sort_key" with type (S)
  */
-public class BasicPutGetExample {
-
-    public static async Task PutItemGetItem()
+public class ItemEncryptDecryptExample
+{
+    public static void PutItemGetItem()
     {
-        var kmsKeyId = TestUtils.TEST_KMS_KEY_ID;
-        var ddbTableName = TestUtils.TEST_DDB_TABLE_NAME;
+        String kmsKeyId = TestUtils.TEST_KMS_KEY_ID;
+        String ddbTableName = TestUtils.TEST_DDB_TABLE_NAME;
+
         // 1. Create a Keyring. This Keyring will be responsible for protecting the data keys that protect your data.
         //    For this example, we will create a AWS KMS Keyring with the AWS KMS Key we want to use.
         //    We will use the `CreateMrkMultiKeyring` method to create this keyring,
@@ -41,13 +45,14 @@ public class BasicPutGetExample {
         //      - ENCRYPT_AND_SIGN: The attribute is encrypted and included in the signature
         //      - SIGN_ONLY: The attribute not encrypted, but is still included in the signature
         //      - DO_NOTHING: The attribute is not encrypted and not included in the signature
-        Dictionary<string, CryptoAction> attributeActionsOnEncrypt = new Dictionary<string, CryptoAction>();
-        attributeActionsOnEncrypt.Add("partition_key",
-            CryptoAction.SIGN_ONLY); // Our partition attribute must be SIGN_ONLY
-        attributeActionsOnEncrypt.Add("sort_key", CryptoAction.SIGN_ONLY); // Our sort attribute must be SIGN_ONLY
-        attributeActionsOnEncrypt.Add("attribute1", CryptoAction.ENCRYPT_AND_SIGN);
-        attributeActionsOnEncrypt.Add("attribute2", CryptoAction.SIGN_ONLY);
-        attributeActionsOnEncrypt.Add(":attribute3", CryptoAction.DO_NOTHING);
+        var attributeActionsOnEncrypt = new Dictionary<String, CryptoAction>
+        {
+            ["partition_key"] = CryptoAction.SIGN_ONLY, // Our partition attribute must be SIGN_ONLY
+            ["sort_key"] = CryptoAction.SIGN_ONLY, // Our sort attribute must be SIGN_ONLY
+            ["attribute1"] = CryptoAction.ENCRYPT_AND_SIGN,
+            ["attribute2"] = CryptoAction.SIGN_ONLY,
+            [":attribute3"] = CryptoAction.DO_NOTHING
+        };
 
         // 3. Configure which attributes we expect to be included in the signature
         //    when reading items. There are two options for configuring this:
@@ -77,12 +82,10 @@ public class BasicPutGetExample {
         //
         //   For this example, we have designed our DynamoDb table such that any attribute name with
         //   the ":" prefix should be considered unauthenticated.
-        const String unsignAttrPrefix = ":";
+        String unsignAttrPrefix = ":";
 
-        // 4. Create the DynamoDb Encryption configuration for the table we will be writing to.
-        Dictionary<String, DynamoDbTableEncryptionConfig> tableConfigs =
-            new Dictionary<String, DynamoDbTableEncryptionConfig>();
-        DynamoDbTableEncryptionConfig config = new DynamoDbTableEncryptionConfig
+        // 4. Create the configuration for the DynamoDb Item Encryptor
+        var config = new DynamoDbItemEncryptorConfig
         {
             LogicalTableName = ddbTableName,
             PartitionKeyName = "partition_key",
@@ -100,56 +103,38 @@ public class BasicPutGetExample {
             //   https://docs.aws.amazon.com/database-encryption-sdk/latest/devguide/supported-algorithms.html
             AlgorithmSuiteId = DBEAlgorithmSuiteId.ALG_AES_256_GCM_HKDF_SHA512_COMMIT_KEY_ECDSA_P384_SYMSIG_HMAC_SHA384
         };
-        tableConfigs.Add(ddbTableName, config);
 
-        // 5. Create a new AWS SDK DynamoDb client using the TableEncryptionConfigs
-        var ddb = new Client.DynamoDbClient(new DynamoDbTablesEncryptionConfig { TableEncryptionConfigs = tableConfigs });
-        
-        // 6. Put an item into our table using the above client.
-        //    Before the item gets sent to DynamoDb, it will be encrypted
-        //    client-side, according to our configuration.
-        Dictionary<String, AttributeValue> item = new Dictionary<String, AttributeValue>();
-        item.Add("partition_key", new AttributeValue("BasicPutGetExample"));
-        item.Add("sort_key", new AttributeValue{N = "0"});
-        item.Add("attribute1", new AttributeValue("encrypt and sign me!"));
-        item.Add("attribute2", new AttributeValue("sign me!"));
-        item.Add(":attribute3", new AttributeValue("ignore me!"));
+        // 5. Create the DynamoDb Item Encryptor
+        var itemEncryptor = new DynamoDbItemEncryptor(config);
 
-        PutItemRequest putRequest = new PutItemRequest
+        // 6. Directly encrypt a DynamoDb item using the DynamoDb Item Encryptor
+        var originalItem = new Dictionary<String, AttributeValue>
         {
-            TableName = ddbTableName,
-            Item = item
+            ["partition_key"] = new AttributeValue("ItemEncryptDecryptExample"),
+            ["sort_key"] = new AttributeValue { N = "0" },
+            ["attribute1"] = new AttributeValue("encrypt and sign me!"),
+            ["attribute2"] = new AttributeValue("sign me!"),
+            [":attribute3"] = new AttributeValue("ignore me!")
         };
 
-        PutItemResponse putResponse = await ddb.PutItemAsync(putRequest);
+        var encryptedItem = itemEncryptor.EncryptItem(
+            new EncryptItemInput { PlaintextItem = originalItem }
+        ).EncryptedItem;
 
-        // Demonstrate that PutItem succeeded
-        Debug.Assert(putResponse.HttpStatusCode == HttpStatusCode.OK);
+        // Demonstrate that the item has been encrypted
+        Debug.Assert(encryptedItem["partition_key"].S.Equals("ItemEncryptDecryptExample"));
+        Debug.Assert(encryptedItem["sort_key"].N.Equals("0"));
+        Debug.Assert(encryptedItem["attribute1"].B != null);
+        Debug.Assert(encryptedItem["attribute1"].S == null);
 
-        // 7. Get the item back from our table using the same client.
-        //    The client will decrypt the item client-side, and return
-        //    back the original item.
-        Dictionary<String, AttributeValue> keyToGet = new Dictionary<String, AttributeValue> ();
-        keyToGet.Add("partition_key", new AttributeValue("BasicPutGetExample"));
-        keyToGet.Add("sort_key", new AttributeValue{N = "0"});
-
-        GetItemRequest getRequest = new GetItemRequest {
-            Key = keyToGet,
-            TableName = ddbTableName,
-            // In this example we configure a strongly consistent read
-            // because we perform a read immediately after a write (for demonstrative purposes).
-            // By default, reads are only eventually consistent.
-            // Read our docs to determine which read consistency to use for your application:
-            // https://docs.aws.amazon.com/amazondynamodb/latest/developerguide/HowItWorks.ReadConsistency.html
-            ConsistentRead = true
-        };
-
-        GetItemResponse getResponse = await ddb.GetItemAsync(getRequest);
+        // 7. Directly decrypt the encrypted item using the DynamoDb Item Encryptor
+        var decryptedItem = itemEncryptor.DecryptItem(
+            new DecryptItemInput { EncryptedItem = encryptedItem }
+        ).PlaintextItem;
 
         // Demonstrate that GetItem succeeded and returned the decrypted item
-        Debug.Assert(getResponse.HttpStatusCode == HttpStatusCode.OK);
-        var returnedItem = getResponse.Item;
-        Debug.Assert(returnedItem["attribute1"].S == "encrypt and sign me!");
+        Debug.Assert(decryptedItem["partition_key"].S.Equals("ItemEncryptDecryptExample"));
+        Debug.Assert(decryptedItem["sort_key"].N.Equals("0"));
+        Debug.Assert(decryptedItem["attribute1"].S.Equals("encrypt and sign me!"));
     }
-
 }
